LoL/Veil.lean
@@ -1,0 +1,248 @@
+import LoL.MProp.Instances
+import LoL.MProp.NonDetT
+
+import LoL.Meta
+
+set_option autoImplicit true
+
+namespace Veil
+
+
+abbrev ExecDet (σ ρ : Type) := ExceptT String (StateT σ Id) ρ
+abbrev Exec (σ ρ : Type) := NonDetT (ExecDet σ) ρ
+
+-- #gen_spec assertE' (σ α : Type) for
+--   wp (m := ExecDet σ) (α := α) (StateT.lift (.mk (.error "assertion failed")))
+open TotalCorrectness in
+#gen_spec Total.getE (σ : Type) for wp (liftM (m := StateT σ Id) (n :=  ExecDet σ) (StateT.get))
+open TotalCorrectness in
+#gen_spec Total.setE (σ : Type) (s : σ) for wp (liftM (m := StateT σ Id) (n :=  ExecDet σ) (StateT.set s))
+open PartialCorrectness in
+#gen_spec Partial.getE (σ : Type) for wp (liftM (m := StateT σ Id) (n :=  ExecDet σ) (StateT.get))
+open PartialCorrectness in
+#gen_spec Partial.setE (σ : Type) (s : σ) for wp (liftM (m := StateT σ Id) (n :=  ExecDet σ) (StateT.set s))
+
+
+
+lemma iInfE : iInf (α := σ -> Prop) f = fun x => ∀ y, f y x := by ext; simp
+lemma iSupE : iSup (α := σ -> Prop) f = fun x => ∃ y, f y x := by ext; simp
+lemma complE : (fᶜ : σ -> Prop) = fun x => ¬ f x := by ext; simp
+
+lemma topE : (⊤ : σ -> Prop) = fun _ => True := by rfl
+lemma botE : (⊥ : σ -> Prop) = fun _ => False := by rfl
+@[simp]
+lemma if_fun [Decidable cnd] (tf ef : α -> β) :
+  (if cnd then fun x => tf x else fun x => ef x) = fun x => if cnd then tf x else ef x := by
+  split_ifs <;> rfl
+@[wpSimp]
+lemma if_app {α β} p [Decidable p] (t e : α -> β)  : (if p then t else e) = fun x => if p then t x else e x := by
+  split <;> rfl
+@[simp]
+lemma not_if {_ : Decidable p} (t e : Prop) : (¬ (if p then t else e)) = if p then ¬ t else ¬ e := by
+  split_ifs <;> simp
+
+def assert (as : Prop) [Decidable as] [Monad m] [MonadExcept String m] : m Unit := do
+  do unless as do throw "assertion failed"
+
+
+lemma assertE {σ} (as : Prop) [Decidable as] :
+  assert (m := Exec σ) as = liftM (assert (m := ExecDet σ) as) := by sorry
+
+lemma pureE {σ ρ} (x : ρ) :
+  pure (f := Exec σ) x = NonDetT.pure x := rfl
+
+section
+-- open Demonic
+-- namespace Demonic
+
+open Demonic TotalCorrectness in
+@[wpSimp]
+lemma wpAssertE [Decidable as] :
+  wp (assert (m := Exec σ) as) post = fun s => as ∧ post .unit s := by
+    simp [assertE, NonDetT.wp_lift]
+    simp [assert]; split_ifs <;> try simp [wpSimp, wp_pure]
+    { ext s; constructor <;> simp_all }
+    simp [throw, throwThe, MonadExceptOf.throw, ExceptT.mk]
+    erw [wp_tot_eq, wp_pure]; simp_all; rfl
+
+open Demonic PartialCorrectness in
+@[wpSimp]
+lemma PartialD.wpAssertE [Decidable as] :
+  wp (assert (m := Exec σ) as) post = fun s => as -> post .unit s := by
+    simp [assertE, NonDetT.wp_lift]
+    simp [assert]; split_ifs <;> try simp [wpSimp, wp_pure]
+    { ext s; constructor <;> simp_all }
+    simp [throw, throwThe, MonadExceptOf.throw, ExceptT.mk]
+    erw [wp_part_eq, wp_pure]; simp_all; rfl
+
+open Angelic TotalCorrectness in
+@[wpSimp]
+lemma wpAssertEA [Decidable as] :
+  wp (assert (m := Exec σ) as) post = fun s => as ∧ post .unit s := by
+    simp [assertE, NonDetT.wp_lift]
+    simp [assert]; split_ifs <;> try simp [wpSimp, wp_pure]
+    { ext s; constructor <;> simp_all }
+    simp [throw, throwThe, MonadExceptOf.throw, ExceptT.mk]
+    erw [wp_tot_eq, wp_pure]; simp_all; rfl
+
+open Angelic PartialCorrectness in
+@[wpSimp]
+lemma PartialD.wpAssertEA [Decidable as] :
+  wp (assert (m := Exec σ) as) post = fun s => as -> post .unit s := by
+    simp [assertE, NonDetT.wp_lift]
+    simp [assert]; split_ifs <;> try simp [wpSimp, wp_pure]
+    { ext s; constructor <;> simp_all }
+    simp [throw, throwThe, MonadExceptOf.throw, ExceptT.mk]
+    erw [wp_part_eq, wp_pure]; simp_all; rfl
+
+open Demonic TotalCorrectness in
+@[wpSimp]
+lemma Total.wpGetE :
+  wp (get (m := Exec σ)) post = fun s => post s s := by
+    ext s; simp only [get, getThe, MonadStateOf.get, @NonDetT.wp_lift, wpSimp]
+
+open Demonic PartialCorrectness in
+@[wpSimp]
+lemma PartialD.wpGetE :
+  wp (get (m := Exec σ)) post = fun s => post s s := by
+    ext s; simp only [get, getThe, MonadStateOf.get, @NonDetT.wp_lift, wpSimp]
+
+open Angelic TotalCorrectness in
+@[wpSimp]
+lemma TotalA.wpGetE :
+  wp (get (m := Exec σ)) post = fun s => post s s := by
+    ext s; simp only [get, getThe, MonadStateOf.get, @NonDetT.wp_lift, wpSimp]
+
+open Angelic PartialCorrectness in
+@[wpSimp]
+lemma PartialA.wpGetE :
+  wp (get (m := Exec σ)) post = fun s => post s s := by
+    ext s; simp only [get, getThe, MonadStateOf.get, @NonDetT.wp_lift, wpSimp]
+
+
+open Demonic TotalCorrectness in
+@[wpSimp]
+lemma Total.wpSetE :
+  wp (set (σ := σ) (m := Exec σ) s) post = fun _ => post .unit s := by
+    ext s; simp only [set, MonadStateOf.set, NonDetT.wp_lift, wpSimp]
+
+open Demonic PartialCorrectness in
+@[wpSimp]
+lemma Partial.wpSetE :
+  wp (set (σ := σ) (m := Exec σ) s) post = fun _ => post .unit s := by
+    ext s; simp only [set, MonadStateOf.set, NonDetT.wp_lift, wpSimp]
+
+open Angelic TotalCorrectness in
+@[wpSimp]
+lemma TotalA.wpSetE :
+  wp (set (σ := σ) (m := Exec σ) s) post = fun _ => post .unit s := by
+    ext s; simp only [set, MonadStateOf.set, NonDetT.wp_lift, wpSimp]
+
+open Angelic PartialCorrectness in
+@[wpSimp]
+lemma PartialA.wpSetE :
+  wp (set (σ := σ) (m := Exec σ) s) post = fun _ => post .unit s := by
+    ext s; simp only [set, MonadStateOf.set, NonDetT.wp_lift, wpSimp]
+
+
+open Demonic TotalCorrectness in
+@[wpSimp]
+lemma Total.wp_if (p : Prop) [Decidable p] (t e : Exec σ α) :
+  wp (if p then t else e) post = fun s => if p then wp t post s else wp e post s := by
+    unfold wp; split_ifs <;> rfl
+
+open Demonic PartialCorrectness in
+@[wpSimp]
+lemma Partial.wp_if (p : Prop) [Decidable p] (t e : Exec σ α) :
+  wp (if p then t else e) post = fun s => if p then wp t post s else wp e post s := by
+    unfold wp; split_ifs <;> rfl
+
+-- end Demonic
+end
+
+
+
+variable {σ ρ : Type}
+
+def nonDet : Exec Nat Unit := do
+  let b₁ <- pick Bool
+  let b₂ <- pick Bool
+  if b₁ then
+    if b₂ then
+      assert False
+    else
+      set ((<-get) + 1)
+  else
+    if b₂ then
+      assume False
+    else
+      set ((<-get) - 1)
+
+example (P : _ -> Prop) : P nonDet.finally := by
+  simp only [nonDet, NonDetT.ite_eq, assertE, pureE]
+  dsimp [bind, NonDetT.pure, NonDetT.finally]
+  unfold NonDetT.bind;
+  simp [set, get, getThe, MonadStateOf.get]
+  unfold NonDetT.ite; dsimp
+  simp [pick_tpc,
+        assume_tpc,
+        lift_tpc,
+        assume_pre,
+        lift_pre,
+        lift_sem,
+        pick_sem,
+        pick_pre,
+        wp_pure,
+        assume_sem,
+        Id, bind_pure
+        ]
+  unfold pick; simp [instMonadNonDetNonDetT, NonDetT.pick]
+  sorry
+
+section
+open Demonic
+
+attribute [wpSimp] wp_bind MonadNonDet.wp_pick MonadNonDet.wp_assume
+
+open TotalCorrectness in
+example (P : _ -> Prop) : P (wp nonDet post) := by
+  simp [nonDet, -NonDetT.ite_eq, wpSimp, iInfE]
+  sorry
+
+open PartialCorrectness in
+example (P : _ -> Prop) : P (wp nonDet post) := by
+  simp [nonDet, -NonDetT.ite_eq, wpSimp, iInfE]
+  sorry
+
+
+end
+
+section
+open Angelic
+
+attribute [wpSimp] wp_bind MonadNonDet.wp_pick MonadNonDet.wp_assume
+
+section
+open TotalCorrectness
+example (P : _ -> Prop) : P (wp nonDet post) := by
+  simp [nonDet, -NonDetT.ite_eq, wpSimp, iSupE]
+  sorry
+
+def tr (c : Exec σ α) (s s' : σ) (r' : α) := wp c (· = r' ∧ · = s') s
+
+example (P : _ -> Prop) : P (tr nonDet s s') := by
+  unfold tr
+  simp [nonDet, -NonDetT.ite_eq, wpSimp, iSupE]
+  sorry
+
+end
+
+open PartialCorrectness in
+example (P : _ -> Prop) : P (wp nonDet post) := by
+  simp [nonDet, -NonDetT.ite_eq, wpSimp, iSupE]
+  sorry
+
+
+end
+
+end Veil
